IPPGrammarTheorems.v
@@ -257,9 +257,9 @@ Qed.
 
 (* Helper tactics for simplifying specific repair terms. *)
 
-(* Simplifies the term [repair_in_2 pr t1 o (InfixNode t21 o2 t22)] *)
-Ltac repair_in_2_inode_destruct pr o t21 o2 t22 :=
-    cbn [repair_in_2] in *;
+(* Simplifies the term [insert_in pr t1 o (InfixNode t21 o2 t22)] *)
+Ltac insert_in_inode_destruct pr o t21 o2 t22 :=
+    cbn [insert_in] in *;
     destruct (is_i_conflict_pattern pr (CR_infix_infix o o2)) eqn:E;
     [ apply is_i_conflict_pattern_true in E |
       apply is_i_conflict_pattern_false in E;
@@ -271,9 +271,9 @@ Ltac repair_in_2_inode_destruct pr o t21 o2 t22 :=
       ]
     ].
 
-(* Simplifies the term [repair_in_2 pr t1 o (PostfixNode t21 o2)] *)
-Ltac repair_in_2_pnode_destruct pr o t21 o2 :=
-    cbn [repair_in_2] in *;
+(* Simplifies the term [insert_in pr t1 o (PostfixNode t21 o2)] *)
+Ltac insert_in_pnode_destruct pr o t21 o2 :=
+    cbn [insert_in] in *;
      destruct (has_infix_lm_conflicts pr o (PostfixNode t21 o2)) eqn:E;
      [apply has_infix_lm_conflicts_true in E |
       assert (forall x, matches_lm (PostfixNode t21 o2) (PostfixPatt HPatt x) ->
@@ -281,9 +281,9 @@ Ltac repair_in_2_pnode_destruct pr o t21 o2 :=
       [apply has_infix_lm_conflicts_false; assumption|]
     ].
 
-(* Simplifies the term [repair_pre pr o (InfixNode t21 o2 t22)] *)
-Ltac repair_pre_inode_destruct pr o t21 o2 t22 :=
-    cbn [repair_pre] in *;
+(* Simplifies the term [insert_pre pr o (InfixNode t21 o2 t22)] *)
+Ltac insert_pre_inode_destruct pr o t21 o2 t22 :=
+    cbn [insert_pre] in *;
     destruct (is_i_conflict_pattern pr (CR_prefix_infix o o2)) eqn:E;
     [ apply is_i_conflict_pattern_true in E |
       apply is_i_conflict_pattern_false in E;
@@ -295,9 +295,9 @@ Ltac repair_pre_inode_destruct pr o t21 o2 t22 :=
       ]
     ].
 
-(* Simplifies the term [repair_pre pr o (PostfixNode t21 o2)] *)
-Ltac repair_pre_pnode_destruct pr o t21 o2 :=
-    cbn [repair_pre] in *;
+(* Simplifies the term [insert_pre pr o (PostfixNode t21 o2)] *)
+Ltac insert_pre_pnode_destruct pr o t21 o2 :=
+    cbn [insert_pre] in *;
      destruct (has_prefix_lm_conflicts pr o (PostfixNode t21 o2)) eqn:E;
      [apply has_prefix_lm_conflicts_true in E |
       assert (forall x, matches_lm (PostfixNode t21 o2) (PostfixPatt HPatt x) ->
@@ -305,9 +305,9 @@ Ltac repair_pre_pnode_destruct pr o t21 o2 :=
       [apply has_prefix_lm_conflicts_false; assumption|]
     ].
 
-(* Simplifies the term [repair_post pr (InfixNode t11 o1 t12) o] *)
-Ltac repair_post_inode_destruct pr t11 o1 t12 o :=
-    cbn [repair_post] in *;
+(* Simplifies the term [insert_post pr (InfixNode t11 o1 t12) o] *)
+Ltac insert_post_inode_destruct pr t11 o1 t12 o :=
+    cbn [insert_post] in *;
     destruct (is_i_conflict_pattern pr (CL_postfix_infix o o1)) eqn:E;
     [ apply is_i_conflict_pattern_true in E |
       apply is_i_conflict_pattern_false in E;
@@ -319,9 +319,9 @@ Ltac repair_post_inode_destruct pr t11 o1 t12 o :=
       ]
     ].
 
-(* Simplifies the term [repair_post pr (PrefixNode o1 t12) o] *)
-Ltac repair_post_pnode_destruct pr o1 t12 o :=
-    cbn [repair_post] in *;
+(* Simplifies the term [insert_post pr (PrefixNode o1 t12) o] *)
+Ltac insert_post_pnode_destruct pr o1 t12 o :=
+    cbn [insert_post] in *;
     destruct (has_postfix_rm_conflicts pr (PrefixNode o1 t12) o) eqn:E;
     [ apply has_postfix_rm_conflicts_true in E |
       assert (forall x, matches_rm (PrefixNode o1 t12) (PrefixPatt x HPatt) ->
@@ -337,47 +337,47 @@ Ltac repair_post_pnode_destruct pr o1 t12 o :=
 
 (* Lemmas that show well-formedness of [repair] *)
 
-Lemma repair_in_2_wf {g} (pr : drules g) t1 o t2 :
+Lemma insert_in_wf {g} (pr : drules g) t1 o t2 :
   wf_parse_tree g t1 -> wf_parse_tree g t2 -> g.(prods) (InfixProd (inl o)) ->
-  wf_parse_tree g (repair_in_2 pr t1 (inl o) t2).
+  wf_parse_tree g (insert_in pr t1 (inl o) t2).
 Proof.
   intros. induction t2.
   - simpl. auto with IPPGrammar.
   - inv H0.
-    repair_in_2_inode_destruct pr (@inl (OPinpre g) (OPpost g) o) t2_1 (@inl (OPinpre g) (OPpost g) o1) t2_2;
+    insert_in_inode_destruct pr (@inl (OPinpre g) (OPpost g) o) t2_1 (@inl (OPinpre g) (OPpost g) o1) t2_2;
     auto with IPPGrammar.
   - simpl. inv H0. auto with IPPGrammar.
   - inv H0.
-    repair_in_2_pnode_destruct pr (@inl (OPinpre g) (OPpost g) o) t2 (@inr (OPinpre g) (OPpost g) o1);
+    insert_in_pnode_destruct pr (@inl (OPinpre g) (OPpost g) o) t2 (@inr (OPinpre g) (OPpost g) o1);
     auto with IPPGrammar.
 Qed.
 
-Lemma repair_pre_wf {g} (pr : drules g) o t2 :
+Lemma insert_pre_wf {g} (pr : drules g) o t2 :
   wf_parse_tree g t2 -> g.(prods) (PrefixProd (inl o)) ->
-  wf_parse_tree g (repair_pre pr (inl o) t2).
+  wf_parse_tree g (insert_pre pr (inl o) t2).
 Proof.
   intros. induction H; eauto with IPPGrammar.
-  - repair_pre_inode_destruct pr (@inl (OPinpre g) (OPpost g) o) t1 (@inl (OPinpre g) (OPpost g) o0) t2;
+  - insert_pre_inode_destruct pr (@inl (OPinpre g) (OPpost g) o) t1 (@inl (OPinpre g) (OPpost g) o0) t2;
     auto with IPPGrammar.
-  - repair_pre_pnode_destruct pr (@inl (OPinpre g) (OPpost g) o) t (@inr (OPinpre g) (OPpost g) o0);
+  - insert_pre_pnode_destruct pr (@inl (OPinpre g) (OPpost g) o) t (@inr (OPinpre g) (OPpost g) o0);
     auto with IPPGrammar.
 Qed.
 
-Lemma repair_in_1_wf {g} (pr : drules g) t1 o t2 :
+Lemma repair_in_wf {g} (pr : drules g) t1 o t2 :
   wf_parse_tree g t1 -> wf_parse_tree g t2 -> g.(prods) (InfixProd (inl o)) ->
-  wf_parse_tree g (repair_in_1 pr t1 (inl o) t2).
+  wf_parse_tree g (repair_in pr t1 (inl o) t2).
 Proof.
-  intro. revert o t2. induction H; intros; simpl; auto using repair_in_2_wf, repair_pre_wf with IPPGrammar.
+  intro. revert o t2. induction H; intros; simpl; auto using insert_in_wf, insert_pre_wf with IPPGrammar.
 Qed.
 
-Lemma repair_post_wf {g} (pr : drules g) t1 o :
+Lemma insert_post_wf {g} (pr : drules g) t1 o :
   wf_parse_tree g t1 -> g.(prods) (PostfixProd (inr o)) ->
-  wf_parse_tree g (repair_post pr t1 (inr o)).
+  wf_parse_tree g (insert_post pr t1 (inr o)).
 Proof.
   intros. induction H; eauto with IPPGrammar.
-  - repair_post_inode_destruct pr t1 (@inl (OPinpre g) (OPpost g) o0) t2 (@inr (OPinpre g) (OPpost g) o);
+  - insert_post_inode_destruct pr t1 (@inl (OPinpre g) (OPpost g) o0) t2 (@inr (OPinpre g) (OPpost g) o);
     auto with IPPGrammar.
-  - repair_post_pnode_destruct pr (@inl (OPinpre g) (OPpost g) o0) t (@inr (OPinpre g) (OPpost g) o);
+  - insert_post_pnode_destruct pr (@inl (OPinpre g) (OPpost g) o0) t (@inr (OPinpre g) (OPpost g) o);
     auto with IPPGrammar.
 Qed.
 
@@ -385,7 +385,7 @@ Lemma repair_wf {g} (pr : drules g) t :
   wf_parse_tree g t ->
   wf_parse_tree g (repair pr t).
 Proof.
-  intro. induction H; simpl; auto using repair_in_1_wf, repair_pre_wf, repair_post_wf with IPPGrammar.
+  intro. induction H; simpl; auto using repair_in_wf, insert_pre_wf, insert_post_wf with IPPGrammar.
 Qed.
 
 (*
@@ -396,49 +396,49 @@ Qed.
 
 (* Lemmas that show yield-preservation of [repair] *)
 
-Lemma repair_pre_yield_preserve {g} (pr : drules g) o t2 :
-  yield (repair_pre pr o t2) = inr o :: yield t2.
+Lemma insert_pre_yield_preserve {g} (pr : drules g) o t2 :
+  yield (insert_pre pr o t2) = inr o :: yield t2.
 Proof.
   induction t2; try reflexivity.
-  - repair_pre_inode_destruct pr o t2_1 o0 t2_2; auto; simpl; rewrite IHt2_1; auto.
-  - repair_pre_pnode_destruct pr o t2 o0; simpl; auto. rewrite IHt2. reflexivity.
+  - insert_pre_inode_destruct pr o t2_1 o0 t2_2; auto; simpl; rewrite IHt2_1; auto.
+  - insert_pre_pnode_destruct pr o t2 o0; simpl; auto. rewrite IHt2. reflexivity.
 Qed.
 
-Lemma repair_in_2_yield_preserve {g} (pr : drules g) t1 o t2 :
-  yield (repair_in_2 pr t1 o t2) = yield t1 ++ inr o :: yield t2.
+Lemma insert_in_yield_preserve {g} (pr : drules g) t1 o t2 :
+  yield (insert_in pr t1 o t2) = yield t1 ++ inr o :: yield t2.
 Proof.
   induction t2; try reflexivity.
-  - repair_in_2_inode_destruct pr o t2_1 o0 t2_2; simpl; auto.
+  - insert_in_inode_destruct pr o t2_1 o0 t2_2; simpl; auto.
     + rewrite IHt2_1. simplify_list_eq. reflexivity.
     + rewrite IHt2_1. simplify_list_eq. reflexivity.
-  - repair_in_2_pnode_destruct pr o t2 o0; simpl; auto. rewrite IHt2. simplify_list_eq. reflexivity.
+  - insert_in_pnode_destruct pr o t2 o0; simpl; auto. rewrite IHt2. simplify_list_eq. reflexivity.
 Qed.
 
-Lemma repair_in_1_yield_preserve {g} (pr : drules g) t1 o t2 :
-  yield (repair_in_1 pr t1 o t2) = yield t1 ++ inr o :: yield t2.
+Lemma repair_in_yield_preserve {g} (pr : drules g) t1 o t2 :
+  yield (repair_in pr t1 o t2) = yield t1 ++ inr o :: yield t2.
 Proof.
   revert o t2. induction t1; intros.
-  - simpl. rewrite repair_in_2_yield_preserve. reflexivity.
+  - simpl. rewrite insert_in_yield_preserve. reflexivity.
   - simplify_list_eq. rewrite <- IHt1_2. rewrite <- IHt1_1. reflexivity.
-  - simpl. rewrite <- IHt1. rewrite repair_pre_yield_preserve. reflexivity.
-  - simpl. rewrite repair_in_2_yield_preserve. reflexivity.
+  - simpl. rewrite <- IHt1. rewrite insert_pre_yield_preserve. reflexivity.
+  - simpl. rewrite insert_in_yield_preserve. reflexivity.
 Qed.
 
-Lemma repair_post_yield_preserve {g} (pr : drules g) t1 o :
-  yield (repair_post pr t1 o) = yield t1 ++ [inr o].
+Lemma insert_post_yield_preserve {g} (pr : drules g) t1 o :
+  yield (insert_post pr t1 o) = yield t1 ++ [inr o].
 Proof.
   induction t1; try reflexivity.
-  - repair_post_inode_destruct pr t1_1 o0 t1_2 o; auto; simplify_list_eq; rewrite IHt1_2; auto.
-  - repair_post_pnode_destruct pr o0 t1 o; auto; simplify_list_eq; rewrite IHt1; auto.
+  - insert_post_inode_destruct pr t1_1 o0 t1_2 o; auto; simplify_list_eq; rewrite IHt1_2; auto.
+  - insert_post_pnode_destruct pr o0 t1 o; auto; simplify_list_eq; rewrite IHt1; auto.
 Qed.
 
 Lemma repair_yield_preserve {g} (pr : drules g) t :
   yield (repair pr t) = yield t.
 Proof.
   induction t; auto; simpl.
-  - rewrite repair_in_1_yield_preserve. rewrite IHt1. rewrite IHt2. reflexivity.
-  - rewrite repair_pre_yield_preserve. rewrite IHt. reflexivity.
-  - rewrite repair_post_yield_preserve. rewrite IHt. reflexivity.
+  - rewrite repair_in_yield_preserve. rewrite IHt1. rewrite IHt2. reflexivity.
+  - rewrite insert_pre_yield_preserve. rewrite IHt. reflexivity.
+  - rewrite insert_post_yield_preserve. rewrite IHt. reflexivity.
 Qed.
 
 (*
@@ -488,52 +488,52 @@ Ltac lcp_cases H :=
 
 (* Proving safety of shallow conflict patterns (i_conflict_patterns). *)
 
-Lemma repair_in_2_top {g} (pr : drules g) t1 o t2 :
-  matches (repair_in_2 pr t1 o t2) (InfixPatt HPatt o HPatt) \/
-  (exists o2, matches t2 (InfixPatt HPatt o2 HPatt) /\ matches (repair_in_2 pr t1 o t2) (InfixPatt HPatt o2 HPatt)) \/
-  (exists o2, matches t2 (PostfixPatt HPatt o2) /\ matches (repair_in_2 pr t1 o t2) (PostfixPatt HPatt o2)).
+Lemma insert_in_top {g} (pr : drules g) t1 o t2 :
+  matches (insert_in pr t1 o t2) (InfixPatt HPatt o HPatt) \/
+  (exists o2, matches t2 (InfixPatt HPatt o2 HPatt) /\ matches (insert_in pr t1 o t2) (InfixPatt HPatt o2 HPatt)) \/
+  (exists o2, matches t2 (PostfixPatt HPatt o2) /\ matches (insert_in pr t1 o t2) (PostfixPatt HPatt o2)).
 Proof.
   destruct t2; eauto 6 with IPPGrammar.
-  - repair_in_2_inode_destruct pr o t2_1 o0 t2_2; eauto 7 with IPPGrammar.
-  - repair_in_2_pnode_destruct pr o t2 o0; eauto 7 with IPPGrammar.
+  - insert_in_inode_destruct pr o t2_1 o0 t2_2; eauto 7 with IPPGrammar.
+  - insert_in_pnode_destruct pr o t2 o0; eauto 7 with IPPGrammar.
 Qed.
 
-Lemma repair_in_2_top_unchanged {g} (pr : drules g) t1 o t2 x :
+Lemma insert_in_top_unchanged {g} (pr : drules g) t1 o t2 x :
   matches_lm t2 (PostfixPatt HPatt x) ->
   lm_conflict_pattern pr (CR_infix_postfix o x) ->
-  (exists o2, matches t2 (InfixPatt HPatt o2 HPatt) /\ matches (repair_in_2 pr t1 o t2) (InfixPatt HPatt o2 HPatt)) \/
-  (exists o2, matches t2 (PostfixPatt HPatt o2) /\ matches (repair_in_2 pr t1 o t2) (PostfixPatt HPatt o2)).
+  (exists o2, matches t2 (InfixPatt HPatt o2 HPatt) /\ matches (insert_in pr t1 o t2) (InfixPatt HPatt o2 HPatt)) \/
+  (exists o2, matches t2 (PostfixPatt HPatt o2) /\ matches (insert_in pr t1 o t2) (PostfixPatt HPatt o2)).
 Proof.
   intros. destruct t2.
   - inv H. inv H1.
   - inv H. inv H1. left.
     eexists. split; auto with IPPGrammar.
-    repair_in_2_inode_destruct pr o t2_1 o0 t2_2; auto with IPPGrammar. exfalso. apply H with x; auto with IPPGrammar.
+    insert_in_inode_destruct pr o t2_1 o0 t2_2; auto with IPPGrammar. exfalso. apply H with x; auto with IPPGrammar.
   - inv H. inv H1.
   - right. eexists. split; auto with IPPGrammar.
-    repair_in_2_pnode_destruct pr o t2 o0; auto with IPPGrammar. exfalso. apply H1 with x; auto.
+    insert_in_pnode_destruct pr o t2 o0; auto with IPPGrammar. exfalso. apply H1 with x; auto.
 Qed.
 
-Lemma repair_in_2_icfree {g} (pr : drules g) t1 o t2 :
+Lemma insert_in_icfree {g} (pr : drules g) t1 o t2 :
   safe_pr pr ->
   i_conflict_free (i_conflict_pattern pr) t1 ->
   i_conflict_free (i_conflict_pattern pr) t2 ->
   (forall o1, i_conflict_pattern pr (CL_infix_infix o o1) -> ~ matches t1 (InfixPatt HPatt o1 HPatt)) ->
-  i_conflict_free (i_conflict_pattern pr) (repair_in_2 pr t1 o t2).
+  i_conflict_free (i_conflict_pattern pr) (insert_in pr t1 o t2).
 Proof.
   intros. induction t2 as [l2|t21 ? o2 t22|o2 t22|t21 ? o2].
   - simpl. apply Infix_cf; auto. intro. inv H3. inv H4. icp_cases H3; inv H5. inv H12. eapply H2; eauto.
-  - repair_in_2_inode_destruct pr o t21 o2 t22.
+  - insert_in_inode_destruct pr o t21 o2 t22.
     + inv H1. apply Infix_cf; auto. intro. inv H1. inv H3. icp_cases H1; inv H4.
       * destruct H6. eexists. eauto with IPPGrammar.
-      * inv H9. decompose [or] (repair_in_2_top pr t1 o t21); rewrite <- H3 in *.
+      * inv H9. decompose [or] (insert_in_top pr t1 o t21); rewrite <- H3 in *.
         **inv H4. eauto using safe_infix_infix.
         **inv H5. inv H4. inv H9. destruct H6. eexists. eauto with IPPGrammar.
         **inv H5. inv H4. inv H9.
     + inv H1. apply Infix_cf; auto with IPPGrammar. intro. inv H1. inv H3. icp_cases H1; inv H4.
       * destruct H6. eexists. eauto with IPPGrammar.
       * inv E2. inv H3. inv H5. inv H3.
-        inv H9. apply repair_in_2_top_unchanged with pr t1 o t21 x2 in H13; auto. destruct H13; rewrite <- H3 in *.
+        inv H9. apply insert_in_top_unchanged with pr t1 o t21 x2 in H13; auto. destruct H13; rewrite <- H3 in *.
         **inv H5. inv H9. inv H10. destruct H6. eexists. eauto with IPPGrammar.
         **inv H5. inv H9. inv H10.
     + apply Infix_cf; auto. intro. inv H4. inv H5. icp_cases H4; inv H6.
@@ -541,74 +541,74 @@ Proof.
       * inv H8. apply H2 with x1; auto with IPPGrammar.
   - simpl. apply Infix_cf; auto with IPPGrammar. intro. inv H3. inv H4. icp_cases H3; inv H5. inv H12. inv H1.
     eapply H2; eauto with IPPGrammar.
-  - repair_in_2_pnode_destruct pr o t21 o2.
+  - insert_in_pnode_destruct pr o t21 o2.
     + inv H1. apply Postfix_cf; auto with IPPGrammar. intro. inv H1. inv H3. icp_cases H1; inv H4. inv H7. inv E.
       inv H4. inv H8.
-      * inv H4. decompose [or] (repair_in_2_top pr t1 o t21); rewrite <- H3 in *.
+      * inv H4. decompose [or] (insert_in_top pr t1 o t21); rewrite <- H3 in *.
         **inv H4. eauto using safe_infix_postfix.
         **inv H8. inv H4. inv H12. destruct H5. eexists. eauto with IPPGrammar.
         **inv H8. inv H4. inv H12.
-      * apply repair_in_2_top_unchanged with pr t1 o t21 x2 in H13; auto. destruct H13; auto; rewrite <- H3 in *.
+      * apply insert_in_top_unchanged with pr t1 o t21 x2 in H13; auto. destruct H13; auto; rewrite <- H3 in *.
         **inv H4. inv H8. inv H10. destruct H5. eexists. eauto with IPPGrammar.
         **inv H4. inv H8. inv H10.
     + apply Infix_cf; auto with IPPGrammar. intro. inv H4. inv H5. icp_cases H4; inv H6. inv H13. inv H8.
       eapply H2; eauto with IPPGrammar.
 Qed.
 
-Lemma repair_pre_top {g} (pr : drules g) o t2 :
-  matches (repair_pre pr o t2) (PrefixPatt o HPatt) \/
-  (exists o2, matches t2 (InfixPatt HPatt o2 HPatt) /\ matches (repair_pre pr o t2) (InfixPatt HPatt o2 HPatt)) \/
-  (exists o2, matches t2 (PostfixPatt HPatt o2) /\ matches (repair_pre pr o t2) (PostfixPatt HPatt o2)).
+Lemma insert_pre_top {g} (pr : drules g) o t2 :
+  matches (insert_pre pr o t2) (PrefixPatt o HPatt) \/
+  (exists o2, matches t2 (InfixPatt HPatt o2 HPatt) /\ matches (insert_pre pr o t2) (InfixPatt HPatt o2 HPatt)) \/
+  (exists o2, matches t2 (PostfixPatt HPatt o2) /\ matches (insert_pre pr o t2) (PostfixPatt HPatt o2)).
 Proof.
   destruct t2; eauto with IPPGrammar.
-  - repair_pre_inode_destruct pr o t2_1 o0 t2_2; eauto 7 with IPPGrammar.
-  - repair_pre_pnode_destruct pr o t2 o0; eauto 7 with IPPGrammar.
+  - insert_pre_inode_destruct pr o t2_1 o0 t2_2; eauto 7 with IPPGrammar.
+  - insert_pre_pnode_destruct pr o t2 o0; eauto 7 with IPPGrammar.
 Qed.
 
-Lemma repair_pre_top_unchanged {g} (pr : drules g) o t2 x :
+Lemma insert_pre_top_unchanged {g} (pr : drules g) o t2 x :
   matches_lm t2 (PostfixPatt HPatt x) ->
   lm_conflict_pattern pr (CR_prefix_postfix o x) ->
-  (exists o2, matches t2 (InfixPatt HPatt o2 HPatt) /\ matches (repair_pre pr o t2) (InfixPatt HPatt o2 HPatt)) \/
-  (exists o2, matches t2 (PostfixPatt HPatt o2) /\ matches (repair_pre pr o t2) (PostfixPatt HPatt o2)).
+  (exists o2, matches t2 (InfixPatt HPatt o2 HPatt) /\ matches (insert_pre pr o t2) (InfixPatt HPatt o2 HPatt)) \/
+  (exists o2, matches t2 (PostfixPatt HPatt o2) /\ matches (insert_pre pr o t2) (PostfixPatt HPatt o2)).
 Proof.
   intros. destruct t2.
   - inv H. inv H1.
   - inv H. inv H1. left.
     eexists. split; auto with IPPGrammar.
-    repair_pre_inode_destruct pr o t2_1 o0 t2_2; auto with IPPGrammar. exfalso. apply H with x; auto with IPPGrammar.
+    insert_pre_inode_destruct pr o t2_1 o0 t2_2; auto with IPPGrammar. exfalso. apply H with x; auto with IPPGrammar.
   - inv H. inv H1.
   - right. eexists. split; auto with IPPGrammar.
-    repair_pre_pnode_destruct pr o t2 o0; auto with IPPGrammar. exfalso. apply H1 with x; auto.
+    insert_pre_pnode_destruct pr o t2 o0; auto with IPPGrammar. exfalso. apply H1 with x; auto.
 Qed.
 
-Lemma repair_pre_icfree {g} (pr : drules g) o t2 :
+Lemma insert_pre_icfree {g} (pr : drules g) o t2 :
   safe_pr pr ->
   i_conflict_free (i_conflict_pattern pr) t2 ->
-  i_conflict_free (i_conflict_pattern pr) (repair_pre pr o t2).
+  i_conflict_free (i_conflict_pattern pr) (insert_pre pr o t2).
 Proof.
   intros. induction t2 as [l2|t21 ? o2 t22|o2 t22|t21 ? o2].
   - simpl. apply Prefix_cf; auto. intro. inv H1. inv H2. icp_cases H1; inv H3. inv H4.
-  - repair_pre_inode_destruct pr o t21 o2 t22.
+  - insert_pre_inode_destruct pr o t21 o2 t22.
     + inv H0. apply Infix_cf; auto. intro. inv H0. inv H1. icp_cases H0; inv H2.
       * inv H12. destruct H4. eexists. eauto with IPPGrammar.
-      * decompose [or] (repair_pre_top pr o t21).
+      * decompose [or] (insert_pre_top pr o t21).
         **inv H7. rewrite <- H2 in *. inv H1.
         **inv H2. inv H1. inv H7. rewrite <- H1 in *. inv H3. destruct H4. eexists. eauto with IPPGrammar.
         **inv H2. inv H1. inv H7. rewrite <- H1 in *. inv H3.
     + inv H0. apply Infix_cf; auto. intro. inv H0. inv H1. inv E2. inv H1. inv H7. inv H1. icp_cases H0; inv H2.
       * destruct H4. eexists. eauto with IPPGrammar.
-      * apply repair_pre_top_unchanged with pr o t21 x0 in H11; auto. destruct H11.
+      * apply insert_pre_top_unchanged with pr o t21 x0 in H11; auto. destruct H11.
         **inv H1. inv H2. inv H8. rewrite <- H2 in *. inv H7. destruct H4. eexists. eauto with IPPGrammar.
         **inv H1. inv H2. inv H8. rewrite <- H2 in *. inv H7.
     + apply Prefix_cf; auto. intro. inv H2. inv H3. icp_cases H2; inv H4. inv H5. contradiction.
   - simpl. apply Prefix_cf; auto. intro. inv H1. inv H2. icp_cases H1; inv H3. inv H4.
-  - repair_pre_pnode_destruct pr o t21 o2.
+  - insert_pre_pnode_destruct pr o t21 o2.
     + inv H0. apply Postfix_cf; auto. inv E. inv H0. intro. inv H0. inv H5. icp_cases H0; inv H6. inv H7. inv H2.
-      * inv H6. decompose [or] (repair_pre_top pr o t21); rewrite <- H5 in *.
+      * inv H6. decompose [or] (insert_pre_top pr o t21); rewrite <- H5 in *.
         ** inv H2.
         ** inv H6. inv H2. inv H8. destruct H3. eexists. eauto with IPPGrammar.
         ** inv H6. inv H2. inv H8.
-      * apply repair_pre_top_unchanged with pr o t21 x in H10; auto.
+      * apply insert_pre_top_unchanged with pr o t21 x in H10; auto.
         destruct H10; rewrite <- H5 in *.
         ** inv H2. inv H6. inv H7. destruct H3. eexists. eauto with IPPGrammar.
         ** inv H2. inv H6. inv H7.
@@ -616,72 +616,72 @@ Proof.
       intro. inv H2. inv H3. icp_cases H2; inv H4. inv H5.
 Qed.
 
-Lemma repair_in_1_icfree {g} (pr : drules g) t1 o t2 :
+Lemma repair_in_icfree {g} (pr : drules g) t1 o t2 :
   safe_pr pr ->
   i_conflict_free (i_conflict_pattern pr) t1 ->
   i_conflict_free (i_conflict_pattern pr) t2 ->
-  i_conflict_free (i_conflict_pattern pr) (repair_in_1 pr t1 o t2).
+  i_conflict_free (i_conflict_pattern pr) (repair_in pr t1 o t2).
 Proof.
   intro. revert o t2. induction t1 as [l1|t11 ? o1 t12|o1 t12|t11 ? o1]; intros; simpl.
-  - apply repair_in_2_icfree; auto with IPPGrammar. intros. intro. inv H3.
+  - apply insert_in_icfree; auto with IPPGrammar. intros. intro. inv H3.
   - inv H0. auto.
-  - inv H0. apply repair_pre_icfree; auto.
-  - apply repair_in_2_icfree; auto with IPPGrammar. intros. intro. inv H3. 
+  - inv H0. apply insert_pre_icfree; auto.
+  - apply insert_in_icfree; auto with IPPGrammar. intros. intro. inv H3. 
 Qed.
 
-Lemma repair_post_top {g} (pr : drules g) t1 o :
-  matches (repair_post pr t1 o) (PostfixPatt HPatt o) \/
-  (exists o1, matches t1 (InfixPatt HPatt o1 HPatt) /\ matches (repair_post pr t1 o) (InfixPatt HPatt o1 HPatt)) \/
-  (exists o1, matches t1 (PrefixPatt o1 HPatt) /\ matches (repair_post pr t1 o) (PrefixPatt o1 HPatt)).
+Lemma insert_post_top {g} (pr : drules g) t1 o :
+  matches (insert_post pr t1 o) (PostfixPatt HPatt o) \/
+  (exists o1, matches t1 (InfixPatt HPatt o1 HPatt) /\ matches (insert_post pr t1 o) (InfixPatt HPatt o1 HPatt)) \/
+  (exists o1, matches t1 (PrefixPatt o1 HPatt) /\ matches (insert_post pr t1 o) (PrefixPatt o1 HPatt)).
 Proof.
   destruct t1; eauto with IPPGrammar.
-  - repair_post_inode_destruct pr t1_1 o0 t1_2 o; eauto 7 with IPPGrammar.
-  - repair_post_pnode_destruct pr o0 t1 o; eauto 7 with IPPGrammar.
+  - insert_post_inode_destruct pr t1_1 o0 t1_2 o; eauto 7 with IPPGrammar.
+  - insert_post_pnode_destruct pr o0 t1 o; eauto 7 with IPPGrammar.
 Qed.
 
-Lemma repair_post_top_unchanged {g} (pr : drules g) t1 o x :
+Lemma insert_post_top_unchanged {g} (pr : drules g) t1 o x :
   matches_rm t1 (PrefixPatt x HPatt) ->
   rm_conflict_pattern pr (CL_postfix_prefix o x) ->
-  (exists o1, matches t1 (InfixPatt HPatt o1 HPatt) /\ matches (repair_post pr t1 o) (InfixPatt HPatt o1 HPatt)) \/
-  (exists o1, matches t1 (PrefixPatt o1 HPatt) /\ matches (repair_post pr t1 o) (PrefixPatt o1 HPatt)).
+  (exists o1, matches t1 (InfixPatt HPatt o1 HPatt) /\ matches (insert_post pr t1 o) (InfixPatt HPatt o1 HPatt)) \/
+  (exists o1, matches t1 (PrefixPatt o1 HPatt) /\ matches (insert_post pr t1 o) (PrefixPatt o1 HPatt)).
 Proof.
   intros. destruct t1.
   - inv H. inv H1.
   - inv H. inv H1. left.
     eexists. split; auto with IPPGrammar.
-    repair_post_inode_destruct pr t1_1 o0 t1_2 o; auto with IPPGrammar. exfalso. apply H with x; auto with IPPGrammar.
+    insert_post_inode_destruct pr t1_1 o0 t1_2 o; auto with IPPGrammar. exfalso. apply H with x; auto with IPPGrammar.
   - right. eexists. split; auto with IPPGrammar.
-    repair_post_pnode_destruct pr o0 t1 o; auto with IPPGrammar. exfalso. apply H1 with x; auto.
+    insert_post_pnode_destruct pr o0 t1 o; auto with IPPGrammar. exfalso. apply H1 with x; auto.
   - inv H. inv H1.
 Qed.
 
-Lemma repair_post_icfree {g} (pr : drules g) t1 o :
+Lemma insert_post_icfree {g} (pr : drules g) t1 o :
   safe_pr pr ->
   i_conflict_free (i_conflict_pattern pr) t1 ->
-  i_conflict_free (i_conflict_pattern pr) (repair_post pr t1 o).
+  i_conflict_free (i_conflict_pattern pr) (insert_post pr t1 o).
 Proof.
   intros. induction t1 as [l1|t11 ? o1 t12|o1 t12|t11 ? o1].
   - simpl. apply Postfix_cf; auto. intro. inv H1. inv H2. icp_cases H1; inv H3. inv H4.
-  - repair_post_inode_destruct pr t11 o1 t12 o.
+  - insert_post_inode_destruct pr t11 o1 t12 o.
     + inv H0. apply Infix_cf; auto. intro. inv H0. inv H1. icp_cases H0; inv H2.
-      * decompose [or] (repair_post_top pr t12 o).
+      * decompose [or] (insert_post_top pr t12 o).
         **inv H12. rewrite <- H2 in *. inv H1.
         **inv H2. inv H1. inv H12. rewrite <- H1 in *. inv H3. destruct H4. eexists. eauto with IPPGrammar.
         **inv H2. inv H1. inv H12. rewrite <- H1 in *. inv H3.
       * inv H12. destruct H4. eexists. eauto with IPPGrammar.
     + inv H0. apply Infix_cf; auto. intro. inv H0. inv H1. inv E2. inv H1. inv H7. inv H1. icp_cases H0; inv H2.
-      * apply repair_post_top_unchanged with pr t12 o x0 in H11; auto. destruct H11.
+      * apply insert_post_top_unchanged with pr t12 o x0 in H11; auto. destruct H11.
         **inv H1. inv H2. inv H7. rewrite <- H2 in *. inv H14. destruct H4. eexists. eauto with IPPGrammar.
         **inv H1. inv H2. inv H7. rewrite <- H2 in *. inv H14.
       * destruct H4. eexists. eauto with IPPGrammar.
     + apply Postfix_cf; auto. intro. inv H2. inv H3. icp_cases H2; inv H4. inv H5. contradiction.
-  - repair_post_pnode_destruct pr o1 t12 o.
+  - insert_post_pnode_destruct pr o1 t12 o.
     + inv H0. apply Prefix_cf; auto. inv E. inv H0. intro. inv H0. inv H5. icp_cases H0; inv H6. inv H7. inv H2.
-      * inv H6. decompose [or] (repair_post_top pr t12 o); rewrite <- H5 in *.
+      * inv H6. decompose [or] (insert_post_top pr t12 o); rewrite <- H5 in *.
         **inv H2.
         **inv H6. inv H2. inv H8. destruct H3. eexists. eauto with IPPGrammar.
         **inv H6. inv H2. inv H8.
-      * apply repair_post_top_unchanged with pr t12 o x in H10; auto.
+      * apply insert_post_top_unchanged with pr t12 o x in H10; auto.
         destruct H10; rewrite <- H5 in *.
         **inv H2. inv H6. inv H7. destruct H3. eexists. eauto with IPPGrammar.
         **inv H2. inv H6. inv H7.
@@ -693,7 +693,7 @@ Lemma repair_icfree {g} (pr : drules g) t :
   safe_pr pr ->
   i_conflict_free (i_conflict_pattern pr) (repair pr t).
 Proof.
-  intro. induction t; simpl; auto using repair_in_1_icfree, repair_pre_icfree, repair_post_icfree with IPPGrammar.
+  intro. induction t; simpl; auto using repair_in_icfree, insert_pre_icfree, insert_post_icfree with IPPGrammar.
 Qed.
 
 
@@ -705,41 +705,41 @@ Qed.
 
 (* Proving safety of deep rm conflict patterns. *)
 
-Lemma repair_in_2_matches_rm {g} (pr : drules g) t1 o1 t2 o2 :
-  matches_rm (repair_in_2 pr t1 o1 t2) (PrefixPatt o2 HPatt) ->
+Lemma insert_in_matches_rm {g} (pr : drules g) t1 o1 t2 o2 :
+  matches_rm (insert_in pr t1 o1 t2) (PrefixPatt o2 HPatt) ->
   matches_rm t2 (PrefixPatt o2 HPatt).
 Proof.
   intros. destruct t2.
   - simpl in H. inv H. inv H0. inv H4. inv H.
-  - repair_in_2_inode_destruct pr o1 t2_1 o t2_2.
+  - insert_in_inode_destruct pr o1 t2_1 o t2_2.
     + inv H. inv H0. auto with IPPGrammar.
     + inv H. inv H0. auto with IPPGrammar.
     + inv H. inv H1. assumption.
   - simpl in H. inv H. inv H0. assumption.
-  - repair_in_2_pnode_destruct pr o1 t2 o.
+  - insert_in_pnode_destruct pr o1 t2 o.
     + inv H. inv H0.
     + inv H. inv H1. inv H5. inv H.
 Qed.
 
-Lemma repair_in_2_drmcfree {g} (pr : drules g) t1 o t2 :
+Lemma insert_in_drmcfree {g} (pr : drules g) t1 o t2 :
   safe_pr pr ->
   drm_conflict_free (rm_conflict_pattern pr) t1 ->
   drm_conflict_free (rm_conflict_pattern pr) t2 ->
   (forall x, rm_conflict_pattern pr (CL_infix_prefix o x) -> ~ matches_rm t1 (PrefixPatt x HPatt)) ->
-  drm_conflict_free (rm_conflict_pattern pr) (repair_in_2 pr t1 o t2).
+  drm_conflict_free (rm_conflict_pattern pr) (insert_in pr t1 o t2).
 Proof.
   intros. induction t2 as [l2|t21 ? o2 t22|o2 t22|t21 ? o2].
   - simpl. apply Infix_drmcf; auto. intro. inv H3. inv H4. rcp_cases H3; inv H5. eapply H2; eauto.
-  - repair_in_2_inode_destruct pr o t21 o2 t22.
+  - insert_in_inode_destruct pr o t21 o2 t22.
     + inv H1. apply Infix_drmcf; auto. intro. inv H1. inv H3. rcp_cases H1; inv H4.
-      destruct H6. eexists. eauto using repair_in_2_matches_rm with IPPGrammar.
+      destruct H6. eexists. eauto using insert_in_matches_rm with IPPGrammar.
     + inv H1. apply Infix_drmcf; auto. intro. inv H1. inv H3. rcp_cases H1; inv H4.
-      destruct H6. eexists. eauto using repair_in_2_matches_rm with IPPGrammar.
+      destruct H6. eexists. eauto using insert_in_matches_rm with IPPGrammar.
     + apply Infix_drmcf; auto with IPPGrammar. intro. inv H4. inv H5. rcp_cases H4; inv H6. eapply H2; eauto.
   - simpl. apply Infix_drmcf; auto with IPPGrammar. intro. inv H3. inv H4. rcp_cases H3; inv H5. eapply H2; eauto.
-  - repair_in_2_pnode_destruct pr o t21 o2.
+  - insert_in_pnode_destruct pr o t21 o2.
     + inv H1. apply Postfix_drmcf; auto. intro. inv H1. inv H3. rcp_cases H1; inv H4.
-      destruct H5. eexists. eauto using repair_in_2_matches_rm with IPPGrammar.
+      destruct H5. eexists. eauto using insert_in_matches_rm with IPPGrammar.
     + apply Infix_drmcf; auto with IPPGrammar. intro. inv H4. inv H5. rcp_cases H4; inv H6. eapply H2; eauto.
 Qed.
 
@@ -749,56 +749,56 @@ Proof.
   apply Prefix_drmcf; auto using Atomic_drmcf. intro. destruct H as [q]. inv H. rcp_cases H0; inv H1.
 Qed.
 
-Lemma repair_pre_matches_rm {g} (pr : drules g) o t2 o2 :
-  matches_rm (repair_pre pr o t2) (PrefixPatt o2 HPatt) ->
+Lemma insert_pre_matches_rm {g} (pr : drules g) o t2 o2 :
+  matches_rm (insert_pre pr o t2) (PrefixPatt o2 HPatt) ->
   matches_rm t2 (PrefixPatt o2 HPatt) \/ o2 = o.
 Proof.
   intros. destruct t2.
   - simpl in H. inv H.
     + inv H0. auto.
     + inv H3. inv H.
-  - repair_pre_inode_destruct pr o t2_1 o0 t2_2.
+  - insert_pre_inode_destruct pr o t2_1 o0 t2_2.
     + inv H. inv H0. left. auto with IPPGrammar.
     + inv H. inv H0. left. auto with IPPGrammar.
     + inv H; auto. inv H1. auto.
   - inv H; auto. inv H0. auto.
-  - repair_pre_pnode_destruct pr o t2 o0.
+  - insert_pre_pnode_destruct pr o t2 o0.
     + inv H. inv H0.
     + inv H; auto. inv H1. auto.
 Qed.
 
-Lemma repair_pre_drmcfree {g} (pr : drules g) o t2 :
+Lemma insert_pre_drmcfree {g} (pr : drules g) o t2 :
   safe_pr pr ->
   drm_conflict_free (rm_conflict_pattern pr) t2 ->
-  drm_conflict_free (rm_conflict_pattern pr) (repair_pre pr o t2).
+  drm_conflict_free (rm_conflict_pattern pr) (insert_pre pr o t2).
 Proof.
   intros. induction t2 as [l2|t21 ? o2 t22|o2 t22|t21 ? o2].
   - simpl. apply prefixnode_single_drmcfree.
-  - repair_pre_inode_destruct pr o t21 o2 t22.
+  - insert_pre_inode_destruct pr o t21 o2 t22.
     + inv H0. apply Infix_drmcf; auto. intro. inv H0. inv H1. rcp_cases H0; inv H2.
-      apply repair_pre_matches_rm in H7. inv H7.
+      apply insert_pre_matches_rm in H7. inv H7.
       * destruct H4. eexists. eauto with IPPGrammar.
       * eapply safe_infix_prefix; eauto using CPrio_infix_prefix.
     + inv H0. apply Infix_drmcf; auto. intro. inv H0. inv H1. rcp_cases H0; inv H2. inv E2. inv H1. inv H3. inv H1.
       destruct t21.
       **inv H11. inv H1.
-      **inv H11. inv H1. rename E into E'. repair_pre_inode_destruct pr o t21_1 o0 t21_2.
+      **inv H11. inv H1. rename E into E'. insert_pre_inode_destruct pr o t21_1 o0 t21_2.
         ***inv H7. inv H1. destruct H4. eexists. eauto with IPPGrammar.
         ***inv H7. inv H1. destruct H4. eexists. eauto with IPPGrammar.
         ***eapply H1; eauto with IPPGrammar.
       **inv H11. inv H1.
-      **rename E into E'. repair_pre_pnode_destruct pr o t21 o0.
+      **rename E into E'. insert_pre_pnode_destruct pr o t21 o0.
         ***inv H7. inv H1.
         ***eapply H1; eauto.
     + apply Prefix_drmcf; auto. intro. inv H2. inv H3. rcp_cases H2; inv H4.
   - simpl. apply Prefix_drmcf; auto. intro. inv H1. inv H2. rcp_cases H1; inv H3.
-  - repair_pre_pnode_destruct pr o t21 o2.
+  - insert_pre_pnode_destruct pr o t21 o2.
     + inv H0. apply Postfix_drmcf; auto. intro. inv H0. inv H1. rcp_cases H0; inv H2. inv E. inv H1. inv H6.
       * inv H1. destruct t21.
         **simpl in H5. inv H5.
           ***inv H1. eauto using safe_prefix_postfix.
           ***inv H9. inv H1.
-        **repair_pre_inode_destruct pr o t21_1 o0 t21_2.
+        **insert_pre_inode_destruct pr o t21_1 o0 t21_2.
           ***inv H5. inv H1. destruct H3. eexists. eauto with IPPGrammar.
           ***inv H5. inv H1. destruct H3. eexists. eauto with IPPGrammar.
           ***inv H5.
@@ -807,21 +807,21 @@ Proof.
         **simpl in H5. inv H5.
           ***inv H1. eauto using safe_prefix_postfix.
           ***destruct H3. eexists. eauto with IPPGrammar.
-        **repair_pre_pnode_destruct pr o t21 o0.
+        **insert_pre_pnode_destruct pr o t21 o0.
           ***inv H5. inv H1.
           ***inv H5.
             ****inv H6. eauto using safe_prefix_postfix.
             ****inv H10. inv H5.
       * destruct t21.
         **inv H9. inv H1.
-        **inv H9. inv H1. repair_pre_inode_destruct pr o t21_1 o0 t21_2.
+        **inv H9. inv H1. insert_pre_inode_destruct pr o t21_1 o0 t21_2.
           ***inv H5. inv H1. destruct H3. eexists. eauto with IPPGrammar.
           ***inv H5. inv H1. destruct H3. eexists. eauto with IPPGrammar.
           ***inv H5.
             ****inv H6. eapply H1; eauto with IPPGrammar.
             ****inv H9. inv H5. destruct H3. eexists. eauto with IPPGrammar.
         **inv H9. inv H1.
-        **repair_pre_pnode_destruct pr o t21 o0.
+        **insert_pre_pnode_destruct pr o t21 o0.
           ***inv H5. inv H1.
           ***eapply H1; eauto.
     + apply Prefix_drmcf; auto. intro. inv H2. inv H3. rcp_cases H2; inv H4.
@@ -833,44 +833,44 @@ Proof.
   apply Postfix_drmcf; auto using Atomic_drmcf. intro. destruct H as [q]. inv H. rcp_cases H0; inv H1. inv H2. inv H.
 Qed.
 
-Lemma repair_post_drmcfree {g} (pr : drules g) t1 o :
+Lemma insert_post_drmcfree {g} (pr : drules g) t1 o :
   safe_pr pr ->
   drm_conflict_free (rm_conflict_pattern pr) t1 ->
-  drm_conflict_free (rm_conflict_pattern pr) (repair_post pr t1 o).
+  drm_conflict_free (rm_conflict_pattern pr) (insert_post pr t1 o).
 Proof.
   intros. induction t1 as [l1|t11 ? o1 t12|o1 t12|t11 ? o1].
   - simpl. apply Postfix_drmcf; auto. intro. inv H1. inv H2. rcp_cases H1; inv H3. inv H4. inv H2.
-  - repair_post_inode_destruct pr t11 o1 t12 o.
+  - insert_post_inode_destruct pr t11 o1 t12 o.
     + inv H0. apply Infix_drmcf; auto. intro. inv H0. inv H1. rcp_cases H0; inv H2.
       destruct H4. eexists. eauto with IPPGrammar.
     + inv H0. apply Infix_drmcf; auto. intro. inv H0. inv H1. rcp_cases H0; inv H2.
       destruct H4. eexists. eauto with IPPGrammar.
     + apply Postfix_drmcf; auto. intro. inv H2. inv H3. rcp_cases H2; inv H4. inv H5. inv H3.
       eapply H1; eauto with IPPGrammar.
-  - repair_post_pnode_destruct pr o1 t12 o.
+  - insert_post_pnode_destruct pr o1 t12 o.
     + inv H0. apply Prefix_drmcf; auto. intro. inv H0. inv H1. rcp_cases H0; inv H2.
     + apply Postfix_drmcf; auto. intro. inv H2. inv H3. rcp_cases H2; inv H4. eapply H1; eauto.
   - simpl. apply Postfix_drmcf; auto. intro. inv H1. inv H2. rcp_cases H1; inv H3. inv H4. inv H2.
 Qed.
 
-Lemma repair_in_1_drmcfree {g} (pr : drules g) t1 o t2 :
+Lemma repair_in_drmcfree {g} (pr : drules g) t1 o t2 :
   safe_pr pr ->
   drm_conflict_free (rm_conflict_pattern pr) t1 ->
   drm_conflict_free (rm_conflict_pattern pr) t2 ->
-  drm_conflict_free (rm_conflict_pattern pr) (repair_in_1 pr t1 o t2).
+  drm_conflict_free (rm_conflict_pattern pr) (repair_in pr t1 o t2).
 Proof.
   intro. revert o t2. induction t1 as [l1|t11 ? o1 t12|o1 t12|t11 ? o1]; intros; simpl.
-  - apply repair_in_2_drmcfree; auto with IPPGrammar. intros. intro. inv H3. inv H4.
+  - apply insert_in_drmcfree; auto with IPPGrammar. intros. intro. inv H3. inv H4.
   - inv H0. auto.
-  - inv H0. apply repair_pre_drmcfree; auto.
-  - apply repair_in_2_drmcfree; auto with IPPGrammar. intros. intro. inv H3. inv H4. 
+  - inv H0. apply insert_pre_drmcfree; auto.
+  - apply insert_in_drmcfree; auto with IPPGrammar. intros. intro. inv H3. inv H4. 
 Qed.
 
 Lemma repair_drmcfree {g} (pr : drules g) t :
   safe_pr pr ->
   drm_conflict_free (rm_conflict_pattern pr) (repair pr t).
 Proof.
-  intro. induction t; simpl; auto using repair_in_1_drmcfree, repair_pre_drmcfree, repair_post_drmcfree with IPPGrammar.
+  intro. induction t; simpl; auto using repair_in_drmcfree, insert_pre_drmcfree, insert_post_drmcfree with IPPGrammar.
 Qed.
 
 (*
@@ -881,15 +881,15 @@ Qed.
 
 (* Proving safety of deep lm conflict patterns. *)
 
-Lemma repair_in_2_dlmcfree {g} (pr : drules g) t1 o t2 :
+Lemma insert_in_dlmcfree {g} (pr : drules g) t1 o t2 :
   safe_pr pr ->
   dlm_conflict_free (lm_conflict_pattern pr) t1 ->
   dlm_conflict_free (lm_conflict_pattern pr) t2 ->
-  dlm_conflict_free (lm_conflict_pattern pr) (repair_in_2 pr t1 o t2).
+  dlm_conflict_free (lm_conflict_pattern pr) (insert_in pr t1 o t2).
 Proof.
   intros. induction t2 as [l2|t21 ? o2 t22|o2 t22|t21 ? o2].
   - simpl. apply Infix_dlmcf; auto. intro. inv H2. inv H3. lcp_cases H2; inv H4. inv H11. inv H3.
-  - repair_in_2_inode_destruct pr o t21 o2 t22.
+  - insert_in_inode_destruct pr o t21 o2 t22.
     + inv H1. apply Infix_dlmcf; auto. intro. inv H1. inv H2. lcp_cases H1; inv H3.
       destruct H5. eexists. eauto with IPPGrammar.
     + inv H1. apply Infix_dlmcf; auto. intro. inv H1. inv H2. lcp_cases H1; inv H3.
@@ -897,19 +897,19 @@ Proof.
     + apply Infix_dlmcf; auto. intro. inv H3. inv H4. lcp_cases H3; inv H5. inv H12. inv H4.
       eapply H2; eauto with IPPGrammar.
   - simpl. apply Infix_dlmcf; auto with IPPGrammar. intro. inv H2. inv H3. lcp_cases H2; inv H4. inv H11. inv H3.
-  - repair_in_2_pnode_destruct pr o t21 o2.
+  - insert_in_pnode_destruct pr o t21 o2.
     + inv H1. apply Postfix_dlmcf; auto. intro. inv H1. inv H2. lcp_cases H1; inv H3.
     + apply Infix_dlmcf; auto with IPPGrammar. intro. inv H3. inv H4. lcp_cases H3; inv H5. eapply H2; eauto.
 Qed.
 
-Lemma repair_pre_dlmcfree {g} (pr : drules g) o t2 :
+Lemma insert_pre_dlmcfree {g} (pr : drules g) o t2 :
   safe_pr pr ->
   dlm_conflict_free (lm_conflict_pattern pr) t2 ->
-  dlm_conflict_free (lm_conflict_pattern pr) (repair_pre pr o t2).
+  dlm_conflict_free (lm_conflict_pattern pr) (insert_pre pr o t2).
 Proof.
   intros. induction t2 as [l2|t21 ? o2 t22|o2 t22|t21 ? o2].
   - simpl. apply Prefix_dlmcf; auto. intro. inv H1. inv H2. lcp_cases H1; inv H3. inv H4. inv H2.
-  - repair_pre_inode_destruct pr o t21 o2 t22.
+  - insert_pre_inode_destruct pr o t21 o2 t22.
     + inv H0. apply Infix_dlmcf; auto. intro. inv H0. inv H1. lcp_cases H0; inv H2.
       destruct H4. eexists. eauto with IPPGrammar.
     + inv H0. apply Infix_dlmcf; auto. intro. inv H0. inv H1. lcp_cases H0; inv H2.
@@ -917,7 +917,7 @@ Proof.
     + apply Prefix_dlmcf; auto. intro. inv H2. inv H3. lcp_cases H2; inv H4. inv H5. inv H3.
       eapply H1; eauto with IPPGrammar.
   - simpl. apply Prefix_dlmcf; auto. intro. inv H1. inv H2. lcp_cases H1; inv H3. inv H4. inv H2.
-  - repair_pre_pnode_destruct pr o t21 o2.
+  - insert_pre_pnode_destruct pr o t21 o2.
     + inv H0. apply Postfix_dlmcf; auto. intro. inv H0. inv H1. lcp_cases H0; inv H2.
     + apply Prefix_dlmcf; auto with IPPGrammar. intro. inv H2. inv H3. lcp_cases H2; inv H4. eapply H1; eauto.
 Qed.
@@ -928,61 +928,61 @@ Proof.
   apply Postfix_dlmcf; auto with IPPGrammar. intro. destruct H as [q]. inv H. lcp_cases H0; inv H1.
 Qed.
 
-Lemma repair_post_matches_lm {g} (pr : drules g) o t1 o1 :
-  matches_lm (repair_post pr t1 o) (PostfixPatt HPatt o1) ->
+Lemma insert_post_matches_lm {g} (pr : drules g) o t1 o1 :
+  matches_lm (insert_post pr t1 o) (PostfixPatt HPatt o1) ->
   matches_lm t1 (PostfixPatt HPatt o1) \/ o1 = o.
 Proof.
   intros. destruct t1.
   - simpl in H. inv H.
     + inv H0. auto.
     + inv H3. inv H.
-  - repair_post_inode_destruct pr t1_1 o0 t1_2 o.
+  - insert_post_inode_destruct pr t1_1 o0 t1_2 o.
     + inv H. inv H0. left. auto with IPPGrammar.
     + inv H. inv H0. left. auto with IPPGrammar.
     + inv H; auto. inv H1. auto.
-  - repair_post_pnode_destruct pr o0 t1 o.
+  - insert_post_pnode_destruct pr o0 t1 o.
     + inv H. inv H0.
     + inv H; auto. inv H1; auto.
   - inv H; auto. inv H0. auto.
 Qed.
 
-Lemma repair_post_dlmcfree {g} (pr : drules g) t1 o :
+Lemma insert_post_dlmcfree {g} (pr : drules g) t1 o :
   safe_pr pr ->
   dlm_conflict_free (lm_conflict_pattern pr) t1 ->
-  dlm_conflict_free (lm_conflict_pattern pr) (repair_post pr t1 o).
+  dlm_conflict_free (lm_conflict_pattern pr) (insert_post pr t1 o).
 Proof.
   intros. induction t1 as [l1|t11 ? o1 t12|o1 t12|t11 ? o1].
   - simpl. apply postfixnode_single_dlmcfree.
-  - repair_post_inode_destruct pr t11 o1 t12 o.
+  - insert_post_inode_destruct pr t11 o1 t12 o.
     + inv H0. apply Infix_dlmcf; auto. intro. inv H0. inv H1. lcp_cases H0; inv H2.
-      apply repair_post_matches_lm in H12. inv H12.
+      apply insert_post_matches_lm in H12. inv H12.
       * destruct H4. eexists. eauto with IPPGrammar.
       * eauto using safe_infix_postfix.
     + inv H0. apply Infix_dlmcf; auto. intro. inv H0. inv H1. lcp_cases H0; inv H2. inv E2. inv H1. inv H3. inv H1.
       destruct t12.
       **inv H11. inv H1.
-      **inv H11. inv H1. rename E into E'. repair_post_inode_destruct pr t12_1 o0 t12_2 o.
+      **inv H11. inv H1. rename E into E'. insert_post_inode_destruct pr t12_1 o0 t12_2 o.
         ***inv H12. inv H1. destruct H4. eexists. eauto with IPPGrammar.
         ***inv H12. inv H1. destruct H4. eexists. eauto with IPPGrammar.
         ***eapply H1; eauto with IPPGrammar.
-      **rename E into E'. repair_post_pnode_destruct pr o0 t12 o.
+      **rename E into E'. insert_post_pnode_destruct pr o0 t12 o.
         ***inv H12. inv H1.
         ***eapply H1; eauto.
       **inv H11. inv H1.
     + apply Postfix_dlmcf; auto. intro. inv H2. inv H3. lcp_cases H2; inv H4.
-  - repair_post_pnode_destruct pr o1 t12 o.
+  - insert_post_pnode_destruct pr o1 t12 o.
     + inv H0. apply Prefix_dlmcf; auto. intro. inv H0. inv H1. lcp_cases H0; inv H2. inv E. inv H1. inv H6.
       * inv H1. destruct t12.
         **simpl in H5. inv H5.
           ***inv H1. eauto using safe_prefix_postfix.
           ***inv H9. inv H1.
-        **repair_post_inode_destruct pr t12_1 o0 t12_2 o.
+        **insert_post_inode_destruct pr t12_1 o0 t12_2 o.
           ***inv H5. inv H1. destruct H3. eexists. eauto with IPPGrammar.
           ***inv H5. inv H1. destruct H3. eexists. eauto with IPPGrammar.
           ***inv H5.
             ****inv H6. eauto using safe_prefix_postfix.
             ****inv H10. inv H5. destruct H3. eexists. eauto with IPPGrammar.
-        **repair_post_pnode_destruct pr o0 t12 o.
+        **insert_post_pnode_destruct pr o0 t12 o.
           ***inv H5. inv H1.
           ***inv H5.
             ****inv H6. eauto using safe_prefix_postfix.
@@ -992,13 +992,13 @@ Proof.
           ***destruct H3. eexists. eauto with IPPGrammar.
       * destruct t12.
         **inv H9. inv H1.
-        **inv H9. inv H1. repair_post_inode_destruct pr t12_1 o0 t12_2 o.
+        **inv H9. inv H1. insert_post_inode_destruct pr t12_1 o0 t12_2 o.
           ***inv H5. inv H1. destruct H3. eexists. eauto with IPPGrammar.
           ***inv H5. inv H1. destruct H3. eexists. eauto with IPPGrammar.
           ***inv H5.
             ****inv H6. eapply H1; eauto with IPPGrammar.
             ****inv H9. inv H5. destruct H3. eexists. eauto with IPPGrammar.
-        **repair_post_pnode_destruct pr o0 t12 o.
+        **insert_post_pnode_destruct pr o0 t12 o.
           ***inv H5. inv H1.
           ***eapply H1; eauto.
         **inv H9. inv H1.
@@ -1006,24 +1006,24 @@ Proof.
   - simpl. apply Postfix_dlmcf; auto. intro. inv H1. inv H2. lcp_cases H1; inv H3.
 Qed.
 
-Lemma repair_in_1_dlmcfree {g} (pr : drules g) t1 o t2 :
+Lemma repair_in_dlmcfree {g} (pr : drules g) t1 o t2 :
   safe_pr pr ->
   dlm_conflict_free (lm_conflict_pattern pr) t1 ->
   dlm_conflict_free (lm_conflict_pattern pr) t2 ->
-  dlm_conflict_free (lm_conflict_pattern pr) (repair_in_1 pr t1 o t2).
+  dlm_conflict_free (lm_conflict_pattern pr) (repair_in pr t1 o t2).
 Proof.
   intro. revert o t2. induction t1 as [l1|t11 ? o1 t12|o1 t12|t11 ? o1]; intros; simpl.
-  - apply repair_in_2_dlmcfree; auto with IPPGrammar.
+  - apply insert_in_dlmcfree; auto with IPPGrammar.
   - inv H0. auto.
-  - inv H0. apply repair_pre_dlmcfree; auto.
-  - apply repair_in_2_dlmcfree; auto with IPPGrammar. 
+  - inv H0. apply insert_pre_dlmcfree; auto.
+  - apply insert_in_dlmcfree; auto with IPPGrammar. 
 Qed.
 
 Lemma repair_dlmcfree {g} (pr : drules g) t :
   safe_pr pr ->
   dlm_conflict_free (lm_conflict_pattern pr) (repair pr t).
 Proof.
-  intro. induction t; simpl; auto using repair_in_1_dlmcfree, repair_pre_dlmcfree, repair_post_dlmcfree with IPPGrammar.
+  intro. induction t; simpl; auto using repair_in_dlmcfree, insert_pre_dlmcfree, insert_post_dlmcfree with IPPGrammar.
 Qed.
 
 (*
@@ -1204,138 +1204,138 @@ Qed.
 
 (* Lemmas showing [repair t] = t if [t] is conflict free *)
 
-Lemma repair_in_2_complete {g} (pr : drules g) t1 o t2 :
+Lemma insert_in_complete {g} (pr : drules g) t1 o t2 :
   complete_pr pr ->
   cfree pr (InfixNode t1 o t2) ->
-  repair_in_2 pr t1 o t2 = InfixNode t1 o t2.
+  insert_in pr t1 o t2 = InfixNode t1 o t2.
 Proof.
   intros. inv H0. inv H2. destruct t2; auto.
-  - repair_in_2_inode_destruct pr o t2_1 o0 t2_2; auto.
+  - insert_in_inode_destruct pr o t2_1 o0 t2_2; auto.
     + inv H1. destruct H6. eexists. eauto with IPPGrammar.
     + inv E2. inv H2. inv H3. destruct H8. eexists. eauto with IPPGrammar.
-  - repair_in_2_pnode_destruct pr o t2 o0; auto. inv E. inv H2. inv H3. destruct H8. eexists. eauto with IPPGrammar.
+  - insert_in_pnode_destruct pr o t2 o0; auto. inv E. inv H2. inv H3. destruct H8. eexists. eauto with IPPGrammar.
 Qed.
 
-Lemma repair_in_2_matches_lm {g} (pr : drules g) t1 o t2 x :
+Lemma insert_in_matches_lm {g} (pr : drules g) t1 o t2 x :
   lm_conflict_pattern pr (CR_infix_postfix o x) ->
   matches_lm t2 (PostfixPatt HPatt x) ->
-  matches_lm (repair_in_2 pr t1 o t2) (PostfixPatt HPatt x).
+  matches_lm (insert_in pr t1 o t2) (PostfixPatt HPatt x).
 Proof.
   intros. induction t2 as [l2|t21 ? o2 t22|o2 t22|t21 ? o2].
   - inv H0. inv H1.
-  - inv H0. inv H1. repair_in_2_inode_destruct pr o t21 o2 t22.
+  - inv H0. inv H1. insert_in_inode_destruct pr o t21 o2 t22.
     + auto with IPPGrammar.
     + inv E2. inv H0. inv H2. inv H0. auto with IPPGrammar.
     + edestruct H0; eauto with IPPGrammar.
   - inv H0. inv H1.
-  - repair_in_2_pnode_destruct pr o t21 o2.
+  - insert_in_pnode_destruct pr o t21 o2.
     + inv H0.
       * inv H1. auto with IPPGrammar.
       * auto with IPPGrammar.
     + edestruct H1; eauto with IPPGrammar.
 Qed.
 
-Lemma repair_in_2_assoc {g} (pr : drules g) t11 o1 t12 o t2 :
+Lemma insert_in_assoc {g} (pr : drules g) t11 o1 t12 o t2 :
   complete_pr pr ->
   cfree pr (InfixNode t11 o1 t12) ->
   ~ i_conflict_pattern pr (CL_infix_infix o o1) ->
-  repair_in_2 pr t11 o1 (repair_in_2 pr t12 o t2) = repair_in_2 pr (InfixNode t11 o1 t12) o t2.
+  insert_in pr t11 o1 (insert_in pr t12 o t2) = insert_in pr (InfixNode t11 o1 t12) o t2.
 Proof.
   intros. assert (H0' := H0). inv H0'. inv H3.
   induction t2 as [l2|t21 ? o2 t22|o2 t22|t21 ? o2].
-  - assert (repair_in_2 pr t12 o (AtomicNode l2) = InfixNode t12 o (AtomicNode l2)); auto. rewrite H3.
-    repair_in_2_inode_destruct pr o1 t12 o (AtomicNode l2).
-    + rewrite repair_in_2_complete; auto.
-    + rewrite repair_in_2_complete; auto.
+  - assert (insert_in pr t12 o (AtomicNode l2) = InfixNode t12 o (AtomicNode l2)); auto. rewrite H3.
+    insert_in_inode_destruct pr o1 t12 o (AtomicNode l2).
+    + rewrite insert_in_complete; auto.
+    + rewrite insert_in_complete; auto.
     + exfalso. destruct H1. auto using complete_neg_1.
-  - repair_in_2_inode_destruct pr o t21 o2 t22.
-    + rewrite <- IHt2_1. rename E into E'. repair_in_2_inode_destruct pr o1 (repair_in_2 pr t12 o t21) o2 t22; auto.
+  - insert_in_inode_destruct pr o t21 o2 t22.
+    + rewrite <- IHt2_1. rename E into E'. insert_in_inode_destruct pr o1 (insert_in pr t12 o t21) o2 t22; auto.
       destruct E. apply complete_trans_4 with o; auto. auto using complete_neg_3.
     + rewrite <- IHt2_1. rename E into E'. rename E2 into E2'.
-      repair_in_2_inode_destruct pr o1 (repair_in_2 pr t12 o t21) o2 t22; auto. exfalso. inv E2'. inv H6. inv H8.
-      inv H6. apply repair_in_2_matches_lm with pr t12 o t21 x in H12; auto. edestruct H3; eauto with IPPGrammar.
+      insert_in_inode_destruct pr o1 (insert_in pr t12 o t21) o2 t22; auto. exfalso. inv E2'. inv H6. inv H8.
+      inv H6. apply insert_in_matches_lm with pr t12 o t21 x in H12; auto. edestruct H3; eauto with IPPGrammar.
       apply complete_trans_7 with o; auto. auto using complete_neg_3.
-    + rename E into E'. rename E2 into E2'. repair_in_2_inode_destruct pr o1 t12 o (InfixNode t21 o2 t22).
-      * rewrite repair_in_2_complete; auto.
+    + rename E into E'. rename E2 into E2'. insert_in_inode_destruct pr o1 t12 o (InfixNode t21 o2 t22).
+      * rewrite insert_in_complete; auto.
       * destruct H1. auto using complete_neg_1.
       * destruct H1. auto using complete_neg_1.
-  - repair_in_2_inode_destruct pr o1 t12 o (PrefixNode o2 t22).
-    + rewrite repair_in_2_complete; auto.
-    + rewrite repair_in_2_complete; auto.
+  - insert_in_inode_destruct pr o1 t12 o (PrefixNode o2 t22).
+    + rewrite insert_in_complete; auto.
+    + rewrite insert_in_complete; auto.
     + destruct H1. auto using complete_neg_1.
-  - repair_in_2_pnode_destruct pr o t21 o2.
-    + rewrite <- IHt2. rename E into E'. repair_in_2_pnode_destruct pr o1 (repair_in_2 pr t12 o t21) o2; auto.
+  - insert_in_pnode_destruct pr o t21 o2.
+    + rewrite <- IHt2. rename E into E'. insert_in_pnode_destruct pr o1 (insert_in pr t12 o t21) o2; auto.
       exfalso. inv E'. inv H6. inv H8.
       * inv H6. edestruct H3; eauto with IPPGrammar. apply complete_trans_7 with o; auto. auto using complete_neg_3.
-      * apply repair_in_2_matches_lm with pr t12 o t21 x in H11; auto. edestruct H3; eauto with IPPGrammar.
+      * apply insert_in_matches_lm with pr t12 o t21 x in H11; auto. edestruct H3; eauto with IPPGrammar.
         apply complete_trans_7 with o; auto. auto using complete_neg_3.
-    + rename E into E'. repair_in_2_inode_destruct pr o1 t12 o (PostfixNode t21 o2).
-      * rewrite repair_in_2_complete; auto.
+    + rename E into E'. insert_in_inode_destruct pr o1 t12 o (PostfixNode t21 o2).
+      * rewrite insert_in_complete; auto.
       * destruct H1. auto using complete_neg_1.
       * destruct H1. auto using complete_neg_1.
 Qed.
 
-Lemma repair_pre_complete {g} (pr : drules g) o t2 :
+Lemma insert_pre_complete {g} (pr : drules g) o t2 :
   cfree pr (PrefixNode o t2) ->
-  repair_pre pr o t2 = PrefixNode o t2.
+  insert_pre pr o t2 = PrefixNode o t2.
 Proof.
   intro. inv H. inv H1. destruct t2 as [l2|t21 o2 t22|o2 t22|t21 o2]; auto.
-  - repair_pre_inode_destruct pr o t21 o2 t22; auto.
+  - insert_pre_inode_destruct pr o t21 o2 t22; auto.
     + inv H0. destruct H4. eexists. eauto with IPPGrammar.
     + inv E2. inv H1. inv H4. inv H1. inv H2. destruct H5. eexists. eauto with IPPGrammar.
-  - repair_pre_pnode_destruct pr o t21 o2; auto. inv E. inv H1. inv H2. destruct H6. eexists. eauto with IPPGrammar.
+  - insert_pre_pnode_destruct pr o t21 o2; auto. inv E. inv H1. inv H2. destruct H6. eexists. eauto with IPPGrammar.
 Qed.
 
-Lemma repair_in_2_prefix {g} (pr : drules g) o1 t12 o t2 :
+Lemma insert_in_prefix {g} (pr : drules g) o1 t12 o t2 :
   complete_pr pr ->
   cfree pr (PrefixNode o1 t12) ->
   ~ rm_conflict_pattern pr (CL_infix_prefix o o1) ->
-  repair_in_2 pr (PrefixNode o1 t12) o t2 = repair_pre pr o1 (repair_in_2 pr t12 o t2).
+  insert_in pr (PrefixNode o1 t12) o t2 = insert_pre pr o1 (insert_in pr t12 o t2).
 Proof.
   intros. assert (H0' := H0). inv H0'. inv H3. induction t2 as [l2|t21 ? o2 t22|o2 t22|t21 ? o2].
-  - cbn [repair_in_2]. repair_pre_inode_destruct pr o1 t12 o (AtomicNode l2).
-    + rewrite repair_pre_complete; auto.
-    + rewrite repair_pre_complete; auto.
+  - cbn [insert_in]. insert_pre_inode_destruct pr o1 t12 o (AtomicNode l2).
+    + rewrite insert_pre_complete; auto.
+    + rewrite insert_pre_complete; auto.
     + destruct E. auto using complete_neg_2.
-  - repair_in_2_inode_destruct pr o t21 o2 t22.
-    + rewrite IHt2_1. rename E into E'. repair_pre_inode_destruct pr o1 (repair_in_2 pr t12 o t21) o2 t22; auto.
+  - insert_in_inode_destruct pr o t21 o2 t22.
+    + rewrite IHt2_1. rename E into E'. insert_pre_inode_destruct pr o1 (insert_in pr t12 o t21) o2 t22; auto.
       destruct E. apply complete_trans_3 with o; auto. auto using complete_neg_2.
     + rewrite IHt2_1. rename E into E', E2 into E2'.
-      repair_pre_inode_destruct pr o1 (repair_in_2 pr t12 o t21) o2 t22; auto. exfalso. inv E2'. inv H6. inv H8. inv H6.
-      apply repair_in_2_matches_lm with pr t12 o t21 x in H12; auto. edestruct H3; eauto with IPPGrammar.
+      insert_pre_inode_destruct pr o1 (insert_in pr t12 o t21) o2 t22; auto. exfalso. inv E2'. inv H6. inv H8. inv H6.
+      apply insert_in_matches_lm with pr t12 o t21 x in H12; auto. edestruct H3; eauto with IPPGrammar.
       apply complete_trans_8 with o; auto. auto using complete_neg_2.
-    + rename E into E', E2 into E2'. repair_pre_inode_destruct pr o1 t12 o (InfixNode t21 o2 t22).
-      * rewrite repair_pre_complete; auto.
-      * rewrite repair_pre_complete; auto.
+    + rename E into E', E2 into E2'. insert_pre_inode_destruct pr o1 t12 o (InfixNode t21 o2 t22).
+      * rewrite insert_pre_complete; auto.
+      * rewrite insert_pre_complete; auto.
       * destruct E. auto using complete_neg_2.
-  - cbn [repair_in_2]. repair_pre_inode_destruct pr o1 t12 o (PrefixNode o2 t22).
-    + rewrite repair_pre_complete; auto.
-    + rewrite repair_pre_complete; auto.
+  - cbn [insert_in]. insert_pre_inode_destruct pr o1 t12 o (PrefixNode o2 t22).
+    + rewrite insert_pre_complete; auto.
+    + rewrite insert_pre_complete; auto.
     + destruct E. auto using complete_neg_2.
-  - repair_in_2_pnode_destruct pr o t21 o2.
-    + rewrite IHt2. rename E into E'. repair_pre_pnode_destruct pr o1 (repair_in_2 pr t12 o t21) o2; auto. exfalso.
+  - insert_in_pnode_destruct pr o t21 o2.
+    + rewrite IHt2. rename E into E'. insert_pre_pnode_destruct pr o1 (insert_in pr t12 o t21) o2; auto. exfalso.
       inv E'. inv H6. inv H8.
       * inv H6. edestruct H3; eauto with IPPGrammar. apply complete_trans_8 with o; auto. auto using complete_neg_2.
-      * apply repair_in_2_matches_lm with pr t12 o t21 x in H11; auto. edestruct H3; eauto with IPPGrammar.
+      * apply insert_in_matches_lm with pr t12 o t21 x in H11; auto. edestruct H3; eauto with IPPGrammar.
         apply complete_trans_8 with o; auto. auto using complete_neg_2.
-    + rename E into E'. repair_pre_inode_destruct pr o1 t12 o (PostfixNode t21 o2).
-      * rewrite repair_pre_complete; auto.
-      * rewrite repair_pre_complete; auto.
+    + rename E into E'. insert_pre_inode_destruct pr o1 t12 o (PostfixNode t21 o2).
+      * rewrite insert_pre_complete; auto.
+      * rewrite insert_pre_complete; auto.
       * destruct E. auto using complete_neg_2.
 Qed.
 
-Lemma repair_in_1_repair_in_2 {g} (pr : drules g) t1 o t2 :
+Lemma repair_in_insert_in {g} (pr : drules g) t1 o t2 :
   complete_pr pr ->
   cfree pr t1 ->
   (forall x1, matches t1 (InfixPatt HPatt x1 HPatt) -> ~ i_conflict_pattern pr (CL_infix_infix o x1)) ->
   (forall x1, matches_rm t1 (PrefixPatt x1 HPatt) -> ~ rm_conflict_pattern pr (CL_infix_prefix o x1)) ->
-  repair_in_1 pr t1 o t2 = repair_in_2 pr t1 o t2.
+  repair_in pr t1 o t2 = insert_in pr t1 o t2.
 Proof.
   unfold cfree. unfold conflict_free. intro. intro.
   revert o t2. induction t1 as [l1|t11 ? o1 t12|o1 t12|t11 ? o1]; intros; simpl; auto.
   - rewrite IHt12.
     + rewrite IHt1_1.
-      * rewrite repair_in_2_assoc; auto. apply H1. auto with IPPGrammar.
+      * rewrite insert_in_assoc; auto. apply H1. auto with IPPGrammar.
       * inv H0. inv H4. inv H3. inv H0. inv H5. auto.
       * intros. inv H3. rename x1 into o11, t1 into t111, t0 into t112. intro. inv H0. inv H4. destruct H10.
         eexists. eauto with IPPGrammar.
@@ -1346,7 +1346,7 @@ Proof.
       eauto with IPPGrammar.
     + intros. apply H2. auto with IPPGrammar.
   - rewrite IHt12.
-    + rewrite repair_in_2_prefix; auto. apply H2. auto with IPPGrammar.
+    + rewrite insert_in_prefix; auto. apply H2. auto with IPPGrammar.
     + inv H0. inv H4. inv H3. inv H0. inv H5. auto.
     + intros. inv H3. rename x1 into o12, t1 into t121, t0 into t122. intro. apply H2 with o1; auto with IPPGrammar.
       apply complete_trans_2 with o12; auto. apply complete_neg_6; auto. intro. inv H0. inv H5. destruct H10. eexists.
@@ -1354,27 +1354,27 @@ Proof.
     + intros. apply H2. auto with IPPGrammar.
 Qed.
 
-Lemma repair_in_1_complete {g} (pr : drules g) t1 o t2 :
+Lemma repair_in_complete {g} (pr : drules g) t1 o t2 :
   complete_pr pr ->
   cfree pr (InfixNode t1 o t2) ->
-  repair_in_1 pr t1 o t2 = InfixNode t1 o t2.
+  repair_in pr t1 o t2 = InfixNode t1 o t2.
 Proof.
-  intros. assert (H0' := H0). inv H0. inv H2. inv H1. inv H0. inv H3. rewrite repair_in_1_repair_in_2; auto.
-  - rewrite repair_in_2_complete; auto.
+  intros. assert (H0' := H0). inv H0. inv H2. inv H1. inv H0. inv H3. rewrite repair_in_insert_in; auto.
+  - rewrite insert_in_complete; auto.
   - unfold cfree. unfold conflict_free. auto.
   - intros. intro. destruct H6. eexists. eauto with IPPGrammar.
   - intros. intro. destruct H5. eexists. eauto with IPPGrammar.
 Qed.
 
-Lemma repair_post_complete {g} (pr : drules g) t1 o :
+Lemma insert_post_complete {g} (pr : drules g) t1 o :
   cfree pr (PostfixNode t1 o) ->
-  repair_post pr t1 o = PostfixNode t1 o.
+  insert_post pr t1 o = PostfixNode t1 o.
 Proof.
   intro. inv H. inv H1. destruct t1 as [l1|t11 o1 t12|o1 t12|t11 o1]; auto.
-  - repair_post_inode_destruct pr t11 o1 t12 o; auto.
+  - insert_post_inode_destruct pr t11 o1 t12 o; auto.
     + inv H0. destruct H4. eexists. eauto with IPPGrammar.
     + inv E2. inv H1. inv H4. inv H1. inv H. destruct H5. eexists. eauto with IPPGrammar.
-  - repair_post_pnode_destruct pr o1 t12 o; auto. inv E. inv H1. inv H. destruct H6. eexists. eauto with IPPGrammar.
+  - insert_post_pnode_destruct pr o1 t12 o; auto. inv E. inv H1. inv H. destruct H6. eexists. eauto with IPPGrammar.
 Qed.
 
 Lemma repair_complete {g} (pr : drules g) t :
@@ -1384,11 +1384,11 @@ Lemma repair_complete {g} (pr : drules g) t :
 Proof.
   intro. induction t; simpl; auto; intros.
   - assert (H0' := H0). inv H0'. inv H2. inv H1. inv H3. inv H4. rewrite IHt1; try split; auto.
-    rewrite IHt2; try split; auto. apply repair_in_1_complete; auto.
+    rewrite IHt2; try split; auto. apply repair_in_complete; auto.
   - assert (H0' := H0). inv H0'. inv H2. inv H1. inv H3. inv H4. rewrite IHt; try split; auto.
-    apply repair_pre_complete; auto.
+    apply insert_pre_complete; auto.
   - assert (H0' := H0). inv H0'. inv H2. inv H1. inv H3. inv H4. rewrite IHt; try split; auto.
-    apply repair_post_complete; auto.
+    apply insert_post_complete; auto.
 Qed.
 
 (*
